<?xml version="1.0" encoding="UTF-8"?>

<rdf:RDF
  xmlns:rdf="http://www.w3.org/1999/02/22-rdf-syntax-ns#"
  xmlns:rdfs="http://www.w3.org/2000/01/rdf-schema#">

<rdfs:Class rdf:ID="Statement">
	<rdfs:comment>A triple consisting of a predicate, a subject, and an object.</rdfs:comment>
</rdfs:Class>

<rdfs:Class rdf:ID="Property">
	<rdfs:comment>A name of a property, defining specific meaning for the property</rdfs:comment>
</rdfs:Class>

<rdfs:Class rdf:ID="Bag">
	<rdfs:comment>An unordered collection</rdfs:comment>
</rdfs:Class>

<rdfs:Class rdf:ID="Seq">
	<rdfs:comment>An ordered collection</rdfs:comment>
</rdfs:Class>

<rdfs:Class rdf:ID="Alt">
	<rdfs:comment>A collection of alternatives</rdfs:comment>
</rdfs:Class>

<rdf:Property rdf:ID="predicate">
	<rdfs:comment>Identifies the property used in a statement when representing the statement in reified form</rdfs:comment>
	<rdfs:domain rdf:resource="#Statement"/>
	<rdfs:range rdf:resource="#Property"/>
</rdf:Property>

<rdf:Property rdf:ID="subject">
	<rdfs:comment>Identifies the resource that a statement is describing when representing the statement in reified form</rdfs:comment>
	<rdfs:domain rdf:resource="#Statement"/>
</rdf:Property>

<rdf:Property rdf:ID="object">
	<rdfs:comment>Identifies the object of a statement when representing the statement in reified form</rdfs:comment>
</rdf:Property>

<rdf:Property rdf:ID="type">
	<rdfs:comment>Identifies the Class of a resource</rdfs:comment>
</rdf:Property>

<rdf:Property rdf:ID="value">
	<rdfs:comment>Identifies the principal value (usually a string) of a property when the property value is a structured resource</rdfs:comment>
</rdf:Property>

</rdf:RDF>
